Update interop printer + memcpy

src/arch/x64/interop/Main.ml
@@ -1,8 +1,8 @@
 open Interop_Printer
 
-(*
+
 let memcpy = ("memcpy", [("dst", TBuffer TUInt64, Sec); ("src", TBuffer TUInt64, Sec)], Stk (Prims.parse_int "0"))
-*)
+
 (* let poly = ("poly", [("ctx", TBuffer TUInt64); ("inp", TBuffer TUInt64); ("len", TBase TUInt64)]) *)
 
 (* let aes = ("aes", [("input_key", TBuffer TUInt128); ("output_key", TBuffer TUInt128)]) *)
@@ -92,7 +92,7 @@ let zero_quad32_buffer = ("zero_quad32_buffer_win", [("b", TBuffer TUInt128, Sec
 let reverse_quad32 = ("reverse_bytes_quad32_buffer_win", [("b", TBuffer TUInt128, Sec)], Stk (Prims.parse_int "0"))
 *)
 
-let name = quad32_xor 
+let name = memcpy 
 
 let _ = print_string (translate_vale X86 name)
 let _ = print_newline()
