src/arch/x64/interop/Memcpy.fst
@@ -8,7 +8,6 @@ module M = LowStar.Modifies
 open LowStar.ModifiesPat
 open FStar.HyperStack.ST
 module HS = FStar.HyperStack
-module S8 = SecretByte
 open Interop
 open Words_s
 open Types_s
@@ -23,12 +22,12 @@ open X64.Vale.Lemmas_i
 module TS = X64.Taint_Semantics_s
 module ME = X64.Memory_i_s
 module BS = X64.Bytes_Semantics_s
-#set-options "--z3rlimit 40"
+#set-options "--z3rlimit 60"
 
 open Vale_memcpy
 
 #set-options "--initial_fuel 5 --max_fuel 5 --initial_ifuel 2 --max_ifuel 2"
-let create_initial_state is_win dst src stack_b (h0:HS.mem{pre_cond h0 dst src /\ B.length stack_b == 24 /\ live h0 stack_b /\ buf_disjoint_from stack_b [dst;src]}) : GTot TS.traceState =
+let create_initial_trusted_state is_win dst src stack_b (h0:HS.mem{pre_cond h0 dst src /\ B.length stack_b == 24 /\ live h0 stack_b /\ buf_disjoint_from stack_b [dst;src]}) : GTot TS.traceState =
   let taint_func (x:b8) : GTot taint =
     if StrongExcludedMiddle.strong_excluded_middle (x == dst) then Secret else
     if StrongExcludedMiddle.strong_excluded_middle (x == src) then Secret else
@@ -40,19 +39,19 @@ let create_initial_state is_win dst src stack_b (h0:HS.mem{pre_cond h0 dst src /
   let addr_stack:nat64 = addrs stack_b + 0 in
   let regs = if is_win then (
     fun r -> begin match r with
-      | Rsp -> addr_stack
-      | Rcx -> addr_dst
-      | Rdx -> addr_src
-      | _ -> init_regs r end)
+    | Rsp -> addr_stack
+    | Rcx -> addr_dst
+    | Rdx -> addr_src
+    | _ -> init_regs r end)
   else (
     fun r -> begin match r with
-      | Rsp -> addr_stack
-      | Rdi -> addr_dst
-      | Rsi -> addr_src
-      | _ -> init_regs r end)
-  in
-  let xmms = init_xmms in
-  let (s_b:BS.state) = {BS.ok = true; BS.regs = regs; BS.xmms = xmms; BS.flags = 0; BS.mem = Interop.down_mem h0 addrs buffers} in
+    | Rsp -> addr_stack
+    | Rdi -> addr_dst
+    | Rsi -> addr_src
+    | _ -> init_regs r end)
+  in let xmms = init_xmms in
+  let (s_b:BS.state) = {BS.ok = true; BS.regs = regs; BS.xmms = xmms; BS.flags = 0;
+       BS.mem = Interop.down_mem h0 addrs buffers} in
   let s0:X64.Memory_i_s.state = {ME.state = s_b; ME.mem = mem} in
   {TS.state = s0; TS.trace = []; TS.memTaint = create_valid_memtaint mem buffers taint_func}
 
@@ -68,23 +67,23 @@ let create_initial_vale_state is_win dst src stack_b (h0:HS.mem{pre_cond h0 dst 
   let addr_stack:nat64 = addrs stack_b + 0 in
   let regs = if is_win then (
     fun r -> begin match r with
-      | Rsp -> addr_stack
-      | Rcx -> addr_dst
-      | Rdx -> addr_src
-      | _ -> init_regs r end)
+    | Rsp -> addr_stack
+    | Rcx -> addr_dst
+    | Rdx -> addr_src
+    | _ -> init_regs r end)
   else (
     fun r -> begin match r with
-      | Rsp -> addr_stack
-      | Rdi -> addr_dst
-      | Rsi -> addr_src
-      | _ -> init_regs r end)
-  in
-  let xmms = init_xmms in
-  {ok = true; regs = regs; xmms = xmms; flags = 0; mem = mem; memTaint =    create_valid_memtaint mem buffers taint_func}
+    | Rsp -> addr_stack
+    | Rdi -> addr_dst
+    | Rsi -> addr_src
+    | _ -> init_regs r end)
+  in let xmms = init_xmms in
+  {ok = true; regs = regs; xmms = xmms; flags = 0; mem = mem;
+      memTaint = create_valid_memtaint mem buffers taint_func}
 
 let create_lemma is_win dst src stack_b (h0:HS.mem{pre_cond h0 dst src /\ B.length stack_b == 24 /\ live h0 stack_b /\ buf_disjoint_from stack_b [dst;src]}) : Lemma
-  (state_of_S (create_initial_state is_win dst src stack_b h0) == create_initial_vale_state is_win dst src stack_b h0) =
-    let s_init = create_initial_state is_win dst src stack_b h0 in
+  (state_of_S (create_initial_trusted_state is_win dst src stack_b h0) == create_initial_vale_state is_win dst src stack_b h0) =
+    let s_init = create_initial_trusted_state is_win dst src stack_b h0 in
     let s0 = state_of_S s_init in
     let s1 = create_initial_vale_state is_win dst src stack_b h0 in
     assert (FunctionalExtensionality.feq s1.regs (regs' s_init.TS.state));
@@ -92,15 +91,16 @@ let create_lemma is_win dst src stack_b (h0:HS.mem{pre_cond h0 dst src /\ B.leng
     lemma_of_ok s_init;
     lemma_of_regs s_init;
     lemma_of_flags s_init;
-    lemma_of_xmms s_init;    
+    lemma_of_xmms s_init;
     lemma_of_mem s_init;
     lemma_of_memTaint s_init;
     ()
 
+// TODO: Prove these two lemmas if they are not proven automatically
 let implies_pre (is_win:bool) (h0:HS.mem) (dst:s8) (src:s8)  (stack_b:b8) : Lemma
   (requires pre_cond h0 dst src /\ B.length stack_b == 24 /\ live h0 stack_b /\ buf_disjoint_from stack_b [dst;src])
   (ensures (
-  B.length stack_b == 24 /\ live h0 stack_b /\ buf_disjoint_from stack_b [dst;src] /\ (
+B.length stack_b == 24 /\ live h0 stack_b /\ buf_disjoint_from stack_b [dst;src] /\ (
   let s0 = create_initial_vale_state is_win dst src stack_b h0 in
   length_t_eq (TBase TUInt64) stack_b;
   length_t_eq (TBase TUInt64) dst;
@@ -114,10 +114,10 @@ let implies_pre (is_win:bool) (h0:HS.mem) (dst:s8) (src:s8)  (stack_b:b8) : Lemm
   ()
 
 let seq_nat64_to_seq_U64 (b:Seq.seq nat64) : (Seq.seq UInt64.t) =
-  Seq.init (Seq.length b) (fun (i:nat { i < Seq.length b }) -> UInt64.uint_to_t (Seq.index b i))
+Seq.init (Seq.length b) (fun (i:nat { i < Seq.length b }) -> UInt64.uint_to_t (Seq.index b i))
 
 let implies_post (is_win:bool) (va_s0:va_state) (va_sM:va_state) (va_fM:va_fuel) (dst:s8) (src:s8)  (stack_b:b8) : Lemma
-  (requires pre_cond va_s0.mem.hs dst src /\ B.length stack_b == 24 /\ live va_s0.mem.hs stack_b /\ buf_disjoint_from stack_b [dst;src] /\
+  (requires pre_cond va_s0.mem.hs dst src /\ B.length stack_b == 24 /\ live va_s0.mem.hs stack_b /\ buf_disjoint_from stack_b [dst;src]/\
     va_post (va_code_memcpy is_win) va_s0 va_sM va_fM is_win stack_b dst src )
   (ensures post_cond va_s0.mem.hs va_sM.mem.hs dst src ) =
   length_t_eq (TBase TUInt64) stack_b;
@@ -127,39 +127,37 @@ let implies_post (is_win:bool) (va_s0:va_state) (va_sM:va_state) (va_fM:va_fuel)
   let src_b = BV.mk_buffer_view src Views.view64 in
   let t = TBase TUInt64 in
   assert (Seq.equal (seq_nat64_to_seq_U64 (buffer_as_seq #t (va_get_mem va_sM) src)) (BV.as_seq va_sM.mem.hs src_b));  
-  assert (Seq.equal (seq_nat64_to_seq_U64 (buffer_as_seq #t (va_get_mem va_sM) dst)) (BV.as_seq va_sM.mem.hs dst_b));  
+  assert (Seq.equal (seq_nat64_to_seq_U64 (buffer_as_seq #t (va_get_mem va_sM) dst)) (BV.as_seq va_sM.mem.hs dst_b));    
   ()
 
-val lemma_ghost_memcpy:  is_win:bool -> dst:s8 -> src:s8 ->  stack_b:b8 -> (h0:HS.mem{pre_cond h0 dst src /\ B.length stack_b == 24 /\ live h0 stack_b /\ buf_disjoint_from stack_b [dst;src]}) ->
+val lemma_ghost_memcpy: is_win:bool -> dst:s8 -> src:s8 ->  stack_b:b8 -> (h0:HS.mem{pre_cond h0 dst src /\ B.length stack_b == 24 /\ live h0 stack_b /\ buf_disjoint_from stack_b [dst;src]}) ->
   Ghost (TS.traceState * nat * HS.mem)
     (requires True)
     (ensures (fun (s1, f1, h1) ->
-      (let s0 = create_initial_state is_win dst src stack_b h0 in
-       Some s1 == TS.taint_eval_code (va_code_memcpy is_win) f1 s0 /\
-       Interop.correct_down h1 addrs [stack_b;dst;src] s1.TS.state.ME.state.BS.mem /\
-       post_cond h0 h1 dst src /\
-       calling_conventions is_win s0 s1)
-      )
-    )
-
+      (let s0 = create_initial_trusted_state is_win dst src stack_b h0 in
+      Some s1 == TS.taint_eval_code (va_code_memcpy is_win) f1 s0 /\
+      Interop.correct_down h1 addrs [stack_b;dst;src] s1.TS.state.ME.state.BS.mem /\
+      post_cond h0 h1 dst src  /\
+      calling_conventions is_win s0 s1)
+    ))
 
 let lemma_ghost_memcpy is_win dst src stack_b h0 =
   length_t_eq (TBase TUInt64) stack_b;
   length_t_eq (TBase TUInt64) dst;
   length_t_eq (TBase TUInt64) src;
-  implies_pre is_win h0 dst src stack_b ;
-  let s0 = create_initial_state is_win dst src stack_b h0 in
+  implies_pre is_win h0 dst src stack_b;
+  let s0 = create_initial_trusted_state is_win dst src stack_b h0 in
   create_lemma is_win dst src stack_b h0;
-  let s_v, f_v = va_lemma_memcpy (va_code_memcpy is_win) (state_of_S s0) is_win stack_b dst src in  
+  let s_v, f_v = va_lemma_memcpy (va_code_memcpy is_win) (state_of_S s0) is_win stack_b dst src  in
   implies_post is_win (state_of_S s0) s_v f_v dst src stack_b;
   Some?.v (TS.taint_eval_code (va_code_memcpy is_win) f_v s0), f_v, s_v.mem.hs
 
 let memcpy dst src  =
   push_frame();
   let (stack_b:b8) = B.alloca (UInt8.uint_to_t 0) (UInt32.uint_to_t 24) in
-  st_put 
-  (fun h -> pre_cond h dst src /\ B.length stack_b == 24 /\ live h stack_b /\ buf_disjoint_from stack_b [dst;src]) 
-  (fun h -> let _, _, h1 = 
+  st_put
+    (fun h -> pre_cond h dst src /\ B.length stack_b == 24 /\ live h stack_b /\ buf_disjoint_from stack_b [dst;src])
+  (fun h -> let _, _, h1 =
     if win then lemma_ghost_memcpy true dst src stack_b h
     else lemma_ghost_memcpy false dst src stack_b h
   in h1);
